rocq-skylabs-cpp2v/tests/phase6_locations.t/no_templates_check.v
@@ -5,7 +5,7 @@ Require Import no_templates_locations.
 Definition generated_uses_indexed_location_dag : bool :=
   match source_locations.(location_data) with
   | ExpandedLocations _ => false
-  | IndexedLocations _ _ => true
+  | IndexedLocations _ _ | CompactIndexedLocations _ _ _ => true
   end.
 
 Example generated_location_storage_is_an_indexed_dag :
@@ -16,12 +16,18 @@ Definition template_symbol_location_count : nat :=
   match source_locations.(location_data) with
   | ExpandedLocations roots => TM.cardinal roots.(msymbol_locations)
   | IndexedLocations _ roots => TM.cardinal roots.(msymbol_locations)
+  | CompactIndexedLocations _ singletons residuals =>
+      List.length singletons.(singleton_msymbol_locations) +
+      TM.cardinal residuals.(msymbol_locations)
   end.
 
 Definition template_type_location_count : nat :=
   match source_locations.(location_data) with
   | ExpandedLocations roots => TM.cardinal roots.(mtype_locations)
   | IndexedLocations _ roots => TM.cardinal roots.(mtype_locations)
+  | CompactIndexedLocations _ singletons residuals =>
+      List.length singletons.(singleton_mtype_locations) +
+      TM.cardinal residuals.(mtype_locations)
   end.
 
 Example template_symbol_locations_are_empty :
